ST/Logic/Formula.v
@@ -1,0 +1,263 @@
+Require Import String.
+Require Import Nat.
+Require Import Lia.
+Require Export Coq.Arith.Compare_dec.
+Require Import Coq.Arith.Peano_dec.
+Require Import Coq.Logic.Eqdep_dec.
+Require Import Coq.Logic.Classical_Pred_Type.
+Require Import Coq.Logic.Classical_Prop.
+Require Import Coq.Vectors.Vector.
+Require Export RelationClasses.
+Require Export Morphisms.
+Require Import List.
+Import ListNotations.
+Open Scope string_scope.
+From ST Require Import EVarsScratchwork Vector.
+From ST Require Export SoftType.
+From ST Require Export Logic.V Logic.Term Logic.Predicate.
+Import VectorNotations.
+(** ** Formulas
+
+The grammar of formulas is rather straightforward. Honestly, I was unsure how
+"slick" I should be: [Verum] could be defined as [Not Falsum], but using a 
+minimal set of connectives seemed _too_ slick for my tastes.
+*)
+Inductive Formula : Type :=
+| Falsum
+| Atom : Predicate -> Formula
+| And : Formula -> Formula -> Formula
+| Or : Formula -> Formula -> Formula
+| Implies : Formula -> Formula -> Formula
+| Exists : Formula -> Formula.
+
+Definition Not (p : Formula) := Implies p Falsum.
+Definition Verum : Formula := Implies Falsum Falsum.
+Definition Forall (p : Formula) := Not (Exists (Not p)).
+
+Fixpoint formula_contains_bvar (index : nat) (A : Formula) : Prop :=
+match A with
+  | Falsum => False
+  | Atom pred => contains_bvar index pred
+  | And fm1 fm2 | Or fm1 fm2 | Implies fm1 fm2 => (formula_contains_bvar index fm1) \/ (formula_contains_bvar index fm2)
+  | Exists fm => (formula_contains_bvar (S index) fm)
+end.
+
+Global Instance ContainsBVarFormula : ContainsBVar Formula := {
+  contains_bvar := formula_contains_bvar
+}.
+
+Fixpoint is_ground_formula (phi : Formula) :=
+match phi with
+| Falsum => True
+| Atom p => is_ground p
+| And f1 f2 | Or f1 f2 | Implies f1 f2 => (is_ground_formula f1) /\ (is_ground_formula f2)
+| Exists f => is_ground_formula f
+end.
+
+Global Instance GroundFormula : Ground Formula := {
+  is_ground := is_ground_formula
+}.
+
+Definition is_sentence (A : Formula) := is_ground_formula A.
+
+(** We can recursively test if two [Formula] objects are identical. This is an
+equality at the level of syntax. *)
+Fixpoint eq_formula (A B : Formula) : bool :=
+match A,B with
+| Falsum, Falsum => true
+| Atom (P n1 s1 args1), Atom (P n2 s2 args2) => 
+      if andb (eqb n1 n2) (eqb s1 s2)
+      then vectors_eqb args1 args2 term_eqb
+      else false
+| And A1 A2, And B1 B2 => andb (eq_formula A1 B1) (eq_formula A2 B2)
+| Or A1 A2, Or B1 B2 => andb (eq_formula A1 B1) (eq_formula A2 B2)
+| Implies A1 A2, Implies B1 B2 =>  andb (eq_formula A1 B1) (eq_formula A2 B2)
+| Exists A1, Exists B1 => eq_formula A1 B1
+| _, _ => false
+end.
+
+Global Instance EqFormula : Eq Formula := {
+  eqb := eq_formula
+}.
+
+Theorem Formula_eq_dec : forall a b : Formula, {a = b} + {a <> b}.
+Proof.
+  decide equality. apply Predicate.eq_dec.
+Defined.
+
+(** "Variable closing", or binding a free variable to a quantifier (or any
+binder), is a bit tricky. We have a helper function here for the iterative
+step. It behaves "functorially", descending to the leafs, i.e., [Falsum] and
+[Atom]. *)
+Fixpoint var_closing_iter (x : name) (n : nat) (phi : Formula) : Formula :=
+match phi with
+| Falsum => phi
+| Atom pred => Atom (subst (FVar x) (Var (BVar n)) pred)
+| And fm1 fm2 => And (var_closing_iter x n fm1) (var_closing_iter x n fm2)
+| Or fm1 fm2 => Or (var_closing_iter x n fm1) (var_closing_iter x n fm2)
+| Implies fm1 fm2 => Implies (var_closing_iter x n fm1) (var_closing_iter x n fm2)
+| Exists fm => Exists (var_closing_iter x (S n) fm)
+end.
+
+Definition quantify (x : name) (phi : Formula) : Formula :=
+  var_closing_iter x 0 phi.
+
+(** Substitution, when replacing a bound variable with an arbitrary term,
+requires care. Why? Because we need to lift the bound variable as we encounter
+quantifiers. 
+
+Particular care must be taken when the term refers to variables or quantities
+in the "context part". Towards that end, we must [lift] the term whenever a
+quantifier is encountered.
+*)
+
+Fixpoint subst_bvar_inner (n : nat) (t : Term) (phi : Formula) : Formula :=
+match phi with
+| Falsum => phi
+| Atom pred => Atom (subst (BVar n) t pred)
+| And fm1 fm2 => And (subst_bvar_inner n t fm1) (subst_bvar_inner n t fm2)
+| Or fm1 fm2 => Or (subst_bvar_inner n t fm1) (subst_bvar_inner n t fm2)
+| Implies fm1 fm2 => Implies (subst_bvar_inner n t fm1) (subst_bvar_inner n t fm2)
+| Exists fm => Exists (subst_bvar_inner (S n) (lift (S n) 1 t) fm)
+end.
+
+(** Specialization and choosing a witness for existential quantification
+amounts to the same "operations" of peeling off an outermost quantifier, then
+behaving as expected. *)
+Fixpoint quantifier_elim_subst (n : nat) (t : Term) (phi : Formula) : Formula :=
+match phi with
+| Exists fm => subst_bvar_inner n t fm
+| And A B => And (quantifier_elim_subst n t A) (quantifier_elim_subst n t B)
+| Or A B => Or (quantifier_elim_subst n t A) (quantifier_elim_subst n t B)
+| Implies A B => Implies (quantifier_elim_subst n t A) (quantifier_elim_subst n t B)
+| _ => phi
+end.
+
+Example subst_bvar_1 : quantifier_elim_subst 0 (Fun "t" []) (Forall (Exists (Atom (P 2 "P" [Var (BVar 0); Var (BVar 1)]))))
+= Not (Not (Exists (Atom (P 2 "P" [Var (BVar 0); Fun "t" []])))).
+Proof.
+  trivial.
+Qed.
+
+Fixpoint lift_formula (c d : nat) (phi : Formula) : Formula :=
+  match phi with
+  | Falsum => phi
+  | Atom pred => Atom (lift c d pred)
+  | And fm1 fm2 => And (lift_formula c d fm1) (lift_formula c d fm2)
+  | Or fm1 fm2 => Or (lift_formula c d fm1) (lift_formula c d fm2)
+  | Implies fm1 fm2 => Implies (lift_formula c d fm1) (lift_formula c d fm2)
+  | Exists fm => Exists (lift_formula (S c) d fm)
+  end.
+
+Global Instance LiftFormula : Lift Formula :=
+{
+  lift := lift_formula
+}.
+(**
+We would encode $\forall x\exists y P(x,y)$ as 
+[Forall (Exists (Atom (P 2 "P" [BVar 1; BVar 0])))], using de Bruijn indices.
+*)
+Check Forall (Exists (Atom (P 2 "P" [Var (BVar 1); Var (BVar 0)]))).
+
+
+(**
+We now have a helper function to quantify over a given variable. They handle
+lifting and replacement, if the variable appears at all in the [Formula]. If
+[n] does not appear in [Formula], then the formula [phi] is returned unchanged.
+*)
+Definition every (n : name) (phi : Formula) : Formula :=
+  let phi' := quantify n (shift phi)
+  in if eqb phi' (shift phi) then phi else Forall phi'.
+
+Definition any (n : name) (phi : Formula) : Formula :=
+  let phi' := quantify n (shift phi)
+  in if eqb phi' (shift phi) then phi else Exists phi'.
+
+(** As a smoke check, we see if variations on a simple formula are "parsed" as
+expected. *)
+Example quantifier_example_1 : (every "x" (any "y" (Atom (P 2 "P" [Var (FVar "x"); Var (FVar "y")]))))
+= Forall (Exists (Atom (P 2 "P" [Var (BVar 1); Var (BVar 0)]))).
+Proof.
+  trivial.
+Qed.
+
+Example quantifier_example_2 : 
+  every "z" (any "y" (Atom (P 2 "P" [Var (FVar "x"); Var (FVar "y")])))
+  = Exists (Atom (P 2 "P" [Var (FVar "x"); Var (BVar 0)])).
+Proof.
+  trivial.
+Qed.
+
+
+Fixpoint fresh_formula (c : Term) (p : Formula) : Prop :=
+  match p with
+  | Falsum => True
+  | Atom phi => fresh c phi
+  | And A B | Or A B | Implies A B => (fresh_formula c A) /\ (fresh_formula c B)
+  | Exists A => fresh_formula c A
+  end.
+  
+Global Instance FreshFormula : Fresh Formula := {
+  fresh := fresh_formula
+}.
+
+Global Instance FreshContext : Fresh (list Formula) := {
+  fresh c Γ := List.Forall (fun fm => fresh c fm) Γ
+}.
+
+(** * Listing the Existential Variables appearing in a Formula *)
+Fixpoint list_evars_formula (phi : Formula) : list nat :=
+match phi with
+| Falsum => []%list
+| Atom pred => list_evars pred
+| And fm1 fm2 | Or fm1 fm2 | Implies fm1 fm2 => insert_merge (list_evars_formula fm1) (list_evars_formula fm2)
+| Exists fm => (list_evars_formula fm)
+end.
+
+Global Instance EnumerateEVarsFormula : EnumerateEVars Formula := {
+list_evars := list_evars_formula
+}. 
+
+Theorem list_evars_formula_sorted : forall (phi : Formula),
+  sorted (list_evars phi).
+Proof. intros. induction phi.
+- simpl; auto. apply sorted_nil.
+- unfold list_evars; unfold EnumerateEVarsFormula. apply list_evars_predicate_sorted.
+- unfold list_evars; unfold EnumerateEVarsFormula.
+  apply insert_merge_sorted2; assumption.
+- unfold list_evars; unfold EnumerateEVarsFormula.
+  apply insert_merge_sorted2; assumption.
+- unfold list_evars; unfold EnumerateEVarsFormula.
+  apply insert_merge_sorted2; assumption.
+- simpl; auto.
+Qed.
+
+Global Instance EnumerateEVarsFormulaList : EnumerateEVars (list Formula) := {
+list_evars Γ := (List.fold_left (fun l' => fun (phi : Formula) => insert_merge (list_evars phi) l')
+ Γ []%list)
+}. 
+
+Theorem list_evars_formula_list_sorted : forall (l : list Formula),
+  sorted (list_evars l).
+Proof.
+  intros. unfold list_evars; unfold EnumerateEVarsFormulaList.
+  apply insert_merge_list_fold_sorted. apply sorted_nil.
+Qed.
+
+Fixpoint shift_evars_formula (phi : Formula) : Formula :=
+match phi with
+| Falsum => phi
+| Atom pred => Atom (shift_evars pred)
+| And fm1 fm2 => And (shift_evars_formula fm1) (shift_evars_formula fm2)
+| Or fm1 fm2 => Or (shift_evars_formula fm1) (shift_evars_formula fm2)
+| Implies fm1 fm2 => Implies (shift_evars_formula fm1) (shift_evars_formula fm2)
+| Exists fm => Exists (shift_evars_formula fm)
+end.
+
+Global Instance ShiftEvarsFormula : ShiftEvars Formula := {
+  shift_evars := shift_evars_formula
+}.
+
+Global Instance ShiftEvarsListFormula : ShiftEvars (list Formula) := {
+  shift_evars Γ := List.map shift_evars Γ
+}.
