ST/Logic/Predicate.v
@@ -1,0 +1,140 @@
+Require Import String.
+Require Import Nat.
+Require Import Lia.
+Require Export Coq.Arith.Compare_dec.
+Require Import Coq.Arith.Peano_dec.
+Require Import Coq.Logic.Eqdep_dec.
+Require Import Coq.Logic.Classical_Pred_Type.
+Require Import Coq.Logic.Classical_Prop.
+Require Import Coq.Vectors.Vector.
+Require Export RelationClasses.
+Require Export Morphisms.
+Require Import List.
+Import ListNotations.
+Open Scope string_scope.
+From ST Require Export SoftType Logic.V Logic.Term.
+From ST Require Import EVarsScratchwork Vector.
+Import VectorNotations.
+(** * Natural Deduction
+
+We need to formalize the proof calculus to then prove the correctness of soft 
+type system.
+
+References relevant:
+
+- https://people.compute.dtu.dk/ahfrom/Formalized%20First-Order%20Logic.pdf
+- https://hal.archives-ouvertes.fr/hal-03096253
+*)
+
+
+Class Ground A : Type := {
+  is_ground : A -> Prop
+}.
+
+Fixpoint is_ground_term (t : Term) :=
+match t with
+| Var x => match x with
+           | FVar _ => True
+           | _ => False
+           end
+| EConst _ => False
+| Fun f args => let fix are_args_ground {k} (ars : Vector.t Term k) :=
+                    match ars with
+                    | [] => True
+                    | a::tl => is_ground_term a /\ are_args_ground tl
+                    end
+                in are_args_ground args
+end.
+
+Global Instance GroundTerm : Ground Term := {
+  is_ground := is_ground_term
+}.
+
+(** ** Predicates
+
+We encode the syntax of a predicate, analogous to [Term], as its arity 
+[n : nat], its [name], and its arguments as a [Vector.t Term].
+*)
+Inductive Predicate : Type := 
+| P : forall (n : nat), name -> Vector.t Term n -> Predicate.
+
+Global Instance ContainsBVarPredicate : ContainsBVar Predicate := {
+  contains_bvar (index : nat) (p : Predicate) :=
+  match p with
+  | P n nm args => Vector.Exists (fun (arg : Term) => contains_bvar index arg)
+                   args
+  end
+}.
+
+Global Instance GroundPredicate : Ground Predicate := {
+  is_ground (p : Predicate) := match p with
+  | P n s args => Vector.Forall is_ground args
+  end
+}.
+
+Global Instance substPred : Subst Predicate :=
+{
+  subst (x : V) (t : Term) (p : Predicate) :=
+  match p with
+  | P n s args => P n s (Vector.map (fun (arg : Term) => subst x t arg) args)
+  end
+}.
+
+Example pred_subst_1 : subst (BVar 0) (Fun "c" []) (P 3 "P" [Var (BVar 1); Var (BVar 0); Fun "f" [Var (BVar 0); Var (FVar "y")]])
+= (P 3 "P" [Var (BVar 1); (Fun "c" []); Fun "f" [(Fun "c" []); Var (FVar "y")]]).
+Proof.
+  trivial.
+Qed.
+
+Global Instance EqPred : Eq Predicate :=
+{
+  eqb (P1 P2 : Predicate) :=
+  match P1,P2 with
+  | P n1 s1 args1, P n2 s2 args2 => 
+      if andb (eqb n1 n2) (eqb s1 s2)
+      then vectors_eqb args1 args2 term_eqb
+      else false
+  end
+}.
+
+(* TODO I am too lazy to prove this... *)
+Lemma eq_dec : forall (x y : Predicate), 
+  {x = y} + {x <> y}.
+Admitted.
+
+Global Instance LiftPred : Lift Predicate :=
+{
+  lift (c d : nat) (p : Predicate) :=
+  match p with
+  | P n s args => P n s (Vector.map (fun (a : Term) => lift c d a) args)
+  end
+}.
+
+Global Instance FreshPredicate : Fresh Predicate := {
+  fresh (c : Term) (p : Predicate) :=
+  match p with
+  | P n s args => Vector.Forall (fun (arg : Term) => fresh c arg) args
+  end
+}.
+
+Global Instance EnumerateEVarsPredicate : EnumerateEVars Predicate := {
+list_evars p := match p with
+| P n s args => Vector.fold_left (fun l' => fun (arg : Term) => insert_merge (list_evars arg) l') []%list args
+end
+}.
+
+Theorem list_evars_predicate_sorted : forall (p : Predicate),
+  sorted (list_evars p).
+Proof. intros.
+  destruct p.
+  rename t into args.
+  unfold list_evars; unfold EnumerateEVarsPredicate.
+  apply insert_merge_vector_fold_sorted2.
+  apply sorted_nil.
+Qed.
+
+Global Instance ShiftEvarsPredicate : ShiftEvars Predicate := {
+shift_evars p := match p with
+| P n s args => P n s (Vector.map shift_evars args)
+end
+}.
