ST/Logic/Term.v
@@ -1,0 +1,710 @@
+Require Import String.
+Require Import Lia.
+Require Import List.
+Require Import Nat.
+Require Import Coq.Vectors.Vector.
+Require Import Coq.Vectors.VectorEq.
+Require Import Coq.Arith.Bool_nat.
+Require Export Coq.Arith.Compare_dec.
+Require Import Coq.Arith.EqNat.
+Require Import Coq.Arith.PeanoNat.
+Require Import Coq.Arith.Peano_dec.
+Require Import Coq.Bool.Bool.
+Require Import Coq.Logic.Classical_Prop.
+Require Import Coq.Logic.Eqdep_dec.
+Require Import Coq.Logic.FunctionalExtensionality.
+Require Export RelationClasses.
+Require Export Morphisms.
+Require Import Program.
+From ST Require Import EVarsScratchwork.
+From ST Require Import Vector.
+From ST Require Import Logic.V.
+Import ListNotations.
+Import VectorNotations.
+Open Scope string_scope.
+(** ** Terms
+
+A [Term] is either a variable, or an n-ary function. Constants are just nullary 
+functions. We do carve out [EConst] for existential constants, to make
+logic easier later on.
+*)
+
+Unset Elimination Schemes.
+Inductive Term : Type :=
+| Var : V -> Term
+| EConst : nat -> Term
+| Fun {n : nat} : name -> Vector.t Term n -> Term.
+
+Definition Term_ind (P : Term -> Prop)
+       (HVar : forall v : V, P (Var v))
+       (HConst : forall n : nat, P (EConst n))
+       (HFun : forall (n : nat) (n0 : name) (t : t Term n),
+         Vector.Forall P t -> P (Fun n0 t))
+       (* ^ extra hypothesis *)
+  : forall t : Term, P t.
+Proof.
+  fix SELF 1; intros [ | | n m t].
+  - apply HVar.
+  - apply HConst.
+  - apply HFun.
+    induction t as [ | ? ? ? IH ]; constructor.
+    + apply SELF.
+    + apply IH.
+Qed.
+
+  Definition Term_rect := 
+fun (P : Term -> Type)
+  (f : forall v : V, P (Var v))
+  (f0 : forall n : nat, P (EConst n))
+  (f1 : forall (n : nat) (n0 : name)
+          (t : t Term n), P (@Fun n n0 t))
+  (t : Term) =>
+match t as t0 return (P t0) with
+| Var v => f v
+| EConst n => f0 n
+| @Fun n n0 t0 => f1 n n0 t0
+end.
+(*
+  Section Term_rect.
+    Variable P : Term -> Type.
+    Variable P_vector : forall n, Vector.t Term n -> Type.
+    Hypothesis P_nil : P_vector 0 []%vector.
+    Hypothesis P_cons : forall {n} t l, P t -> P_vector n l -> P_vector (S n) (t :: l)%vector.
+    Hypothesis P_Var : forall a, P (Var a).
+    Hypothesis P_EConst : forall n, P (EConst n).
+    Hypothesis P_Fun : forall {n} nm l, P_vector n l -> P (@Fun n nm l).
+Print list_rect.
+    Fixpoint Term_rect (t : Term) : P t :=
+      let fix go_vector {n} (l : Vector.t Term n) : P_vector n l :=
+          match l with
+          | []%vector => P_nil
+          | (t :: l)%vector => P_cons t l (Term_rect t) (go_vector l) (* (Term_rect t) (go_vector l) *)
+          end
+      in
+      match t with
+      | Var x => P_Var x
+      | EConst n => P_EConst n
+      | Fun nm args => P_Fun nm args (go_vector args)
+      end.
+  End Term_rect.
+*)
+(*
+  Section Term_rect.
+    Variable P : Term -> Type.
+    Variable P_vector : forall n, Vector.t Term n -> Type.
+    Hypothesis P_nil : P_vector 0 []%vector.
+    Hypothesis P_cons : forall {n} t l, P t -> P_vector n l -> P_vector (S n) (t :: l)%vector.
+    Hypothesis P_Var : forall a, P (Var a).
+    Hypothesis P_EConst : forall n, P (EConst n).
+    Hypothesis P_Fun : forall {n} nm l, P_vector n l -> P (@Fun n nm l).
+Print list_rect.
+    Fixpoint Term_rect (t : Term) : P t :=
+      let fix go_vector {n} (l : Vector.t Term n) : P_vector n l :=
+          match l with
+          | []%vector => P_nil
+          | (t :: l)%vector => P_cons t l (Term_rect t) (go_vector l) (* (Term_rect t) (go_vector l) *)
+          end
+      in
+      match t with
+      | Var x => P_Var x
+      | EConst n => P_EConst n
+      | Fun nm args => P_Fun nm args (go_vector args)
+      end.
+  End Term_rect.
+*)
+Set Elimination Schemes.
+
+Definition constant (c : name) : Term :=
+@Fun 0 c [].
+
+Fixpoint term_eqb (t1 t2 : Term) : bool :=
+match t1,t2 with
+| Var x1, Var x2 => eqb x1 x2
+| EConst n1, EConst n2 => eqb n1 n2
+| @Fun n1 s1 args1, @Fun n2 s2 args2 => 
+  (* eqb n1 n2 && eqb s1 s2 && (Vector.eqb Term term_eqb args1 args2) *)
+  let fix args_eqb {n1 n2} (ar1 : Vector.t Term n1) (ar2 : Vector.t Term n2) : bool :=
+      match ar1,ar2 with
+      | Vector.nil _, Vector.nil _ => true
+      | Vector.cons _ h1 k1 t1,  Vector.cons _ h2 k2 t2 => (andb (term_eqb h1 h2) (args_eqb t1 t2))
+      | _, _ => false
+      end
+  in (eqb n1 n2) && (eqb s1 s2) && (args_eqb args1 args2) 
+| _, _ => false
+end.
+
+Fixpoint args_eqb {n1 n2} (ar1 : Vector.t Term n1) (ar2 : Vector.t Term n2) : bool :=
+match ar1,ar2 with
+| Vector.nil _, Vector.nil _ => true
+| Vector.cons _ h1 k1 t1,  Vector.cons _ h2 k2 t2 => (andb (term_eqb h1 h2) (args_eqb t1 t2))
+| _, _ => false
+end.
+
+Global Instance EqTerm : Eq Term := {
+  eqb := term_eqb
+}.
+
+(*
+Require Import Coq.Vectors.VectorSpec.
+Lemma args_eqb_length (n1 n2 : nat) (args1 : Vector.t Term n1) (args2 : Vector.t Term n2) :
+  n1 <> n2 -> args_eqb (args1) (args2) = false.
+Proof.
+  intros. apply Coq.Arith.Compare_dec.not_eq in H.
+  destruct H.
+  - set (n := min n1 n2).
+    assert (n = n1). lia. 
+    set (k := n2 - n).
+    assert (n2 = n + k). lia.
+    revert args2. rewrite H1.
+    revert args1. assert(n + 0 = n1). lia. rewrite <- H2.
+    intros.
+    set (vs := (@Vector.splitat Term n k args2)).
+    set (us := (@Vector.splitat Term n 0 args1)).
+    destruct vs as [ls2 tls2]. destruct us as [ls1 tls1].
+    assert ({args_eqb ls1 ls2 = true} + {args_eqb ls1 ls2 <> true}). { decide equality. }
+    destruct H3.
+    + 
+    apply min_l in H as H1.
+    Vector.splitat(n, 
+*)
+
+Lemma args_eqb_ind (n : nat) (h1 h2 : Term) (args1 args2 : Vector.t Term n) :
+  args_eqb (h1::args1) (h2::args2)
+  = (eqb h1 h2) && (args_eqb args1 args2).
+Proof.
+  intros. unfold args_eqb; unfold EqTerm; unfold term_eqb. simpl; auto.
+Qed.
+
+(*
+Require Import Coq.Arith.EqNat.
+Lemma args_eqb_ind2 (n1 n2 : nat) (h1 h2 : Term) (args1 : Vector.t Term n1) (args2 : Vector.t Term n2) :
+  args_eqb (h1::args1) (h2::args2)
+  = (eqb n1 n2) && (eqb h1 h2) && (args_eqb args1 args2).
+Proof.
+  intros. assert ({n1 = n2} + {n1 <> n2}). decide equality. destruct H.
+  - revert args1; revert args2. rewrite e. intros.
+    assert (args_eqb (h1::args1) (h2::args2) = (eqb h1 h2) && (args_eqb args1 args2)). {
+      apply args_eqb_ind.
+    }
+    assert (eqb n2 n2 = true). apply Nat.eqb_refl. rewrite H0.
+    rewrite H. unfold andb; simpl; auto.
+  - 
+    
+  induction args1.
+  - destruct args2.
+  + unfold args_eqb; unfold EqTerm; unfold term_eqb. simpl; auto.
+  + simpl; auto. unfold args_eqb. apply andb_false_r.
+  - induction args2.
+  + simpl; auto. unfold args_eqb. apply andb_false_r.
+  +
+    assert (eqb (S n) (S n0) && eqb h1 h2 && args_eqb (h :: args1) (h0 :: args2)
+            
+   reflexivity. simpl; auto.
+    unfold args_eqb; unfold EqTerm; unfold term_eqb. simpl; auto.
+Qed.
+*)
+Lemma fun_eqb (n : nat) (s1 s2 : name) (args1 args2 : Vector.t Term n) :
+  eqb (Fun s1 args1) (Fun s2 args2) =
+  (eqb n n) && (eqb s1 s2) && (args_eqb args1 args2).
+Proof.
+  unfold eqb; unfold EqTerm; unfold term_eqb.
+  unfold andb. simpl; auto.
+Qed.
+
+Lemma fun_eqb2 (n1 n2 : nat) (s1 s2 : name) (args1 : Vector.t Term n1) (args2 : Vector.t Term n2) :
+  eqb (Fun s1 args1) (Fun s2 args2) =
+  (eqb n1 n2) && (eqb s1 s2) && (args_eqb args1 args2).
+Proof.
+  unfold eqb; unfold EqTerm; unfold term_eqb.
+  unfold andb. simpl; auto.
+Qed.
+
+Lemma constant_eqb_refl (s : name) : eqb (Fun s []) (Fun s []) = true.
+Proof.
+  intros.
+  assert ((eqb s s) = true). apply String.eqb_refl.
+  assert ((eqb 0 0) = true). unfold eqb; apply Nat.eqb_refl.
+  unfold eqb; unfold EqTerm; unfold term_eqb.
+  rewrite H; rewrite H0. unfold andb. reflexivity.
+Qed.
+
+Lemma fun_eqb_step (n : nat) (n0 : name) (t : Vector.t Term n) (h : Term) 
+  (IH : Forall (fun t : Term => eqb t t = true) t ->
+        (forall a : Term, VectorDef.In a t -> (fun t : Term => eqb t t = true) a) ->
+        eqb n n = true -> eqb (Fun n0 t) (Fun n0 t) = true) :
+  Forall (fun t : Term => eqb t t = true) (h :: t) -> eqb (Fun n0 (h :: t)) (Fun n0 (h :: t)) = true.
+Proof.
+  intros. set (P := (fun t : Term => eqb t t = true)). fold P in H.
+  assert (forall a : Term, VectorDef.In a (h :: t) -> P a). {
+    apply (Vector.Forall_forall Term P (S n) (h::t)).
+    assumption.
+  }
+  assert (Forall P (h :: t)) as IH1. assumption.
+  apply Vector_Forall_cons_iff in IH1. destruct IH1.
+  assert (forall a : Term, VectorDef.In a t -> P a). {
+    apply (Vector.Forall_forall Term P n t).
+    assumption.
+  }
+  fold P in IH.
+  assert (eqb (Fun n0 t) (Fun n0 t) = true). {
+    apply IH. assumption. assumption. apply Nat.eqb_refl.
+  }
+  unfold P in H1.
+  
+  assert (eqb (@Fun (S n) n0 (h :: t)) (@Fun (S n) n0 (h :: t)) = 
+          ((eqb (S n) (S n)) && (eqb n0 n0) &&
+            (args_eqb (h :: t) (h :: t)))). {
+    apply fun_eqb.
+  }
+  rewrite H5. 
+  assert (eqb (S n) (S n) = true). apply Nat.eqb_refl.
+  rewrite H6.
+  assert (eqb n0 n0 = true). apply String.eqb_refl.
+  rewrite H7. unfold andb.
+  
+  assert (args_eqb (h :: t) (h :: t) = 
+          eqb h h && args_eqb t t). {
+    apply args_eqb_ind.
+  }
+  rewrite H8. rewrite H1. unfold andb.
+  
+  assert (eqb (@Fun n n0 t) (@Fun n n0 t) = 
+          ((eqb n n) && (eqb n0 n0) &&
+            (args_eqb t t))). {
+    apply fun_eqb.
+  }
+  assert (eqb n n = true). apply Nat.eqb_refl.
+  rewrite H7 in H9. rewrite H10 in H9. unfold andb in H9.
+  rewrite H9 in H4. assumption.
+Qed.
+
+Theorem term_eqb_refl (t : Term) : eqb t t = true.
+Proof.
+  induction t.
+  - unfold eqb; apply V_eqb_refl.
+  - unfold eqb; apply Nat.eqb_refl.
+  - set (P := (fun t : Term => eqb t t = true)).
+    fold P in H. Check Vector.Forall_forall.
+    assert (forall a : Term, VectorDef.In a t -> P a). {
+      apply (Vector.Forall_forall Term P n t). assumption.
+    }
+    assert ((eqb n n) = true). unfold eqb; apply Nat.eqb_refl.
+    assert ((eqb n0 n0) = true). apply String.eqb_refl.
+    induction t.
+    apply (constant_eqb_refl n0).
+    apply fun_eqb_step. assumption. assumption.
+Qed.
+
+(*
+Theorem term_eqb_eq (t1 t2 : Term) : eqb t1 t2 = true -> t1 = t2.
+Proof.
+  intros. induction t1.
+  - unfold eqb in H; unfold EqTerm in H; unfold term_eqb in H. destruct t2.
+  + apply V_eqb_eq in H. rewrite H; reflexivity.
+  + discriminate.
+  + discriminate.
+  - unfold eqb in H; unfold EqTerm in H; unfold term_eqb in H. destruct t2. discriminate.
+    apply Nat.eqb_eq in H. rewrite H; reflexivity. discriminate.
+  - destruct t2. discriminate. discriminate.
+    assert (eqb (Fun n0 t) (Fun n2 t0)
+            = eqb n n1 && eqb n0 n2 && args_eqb t t0). {
+      apply (fun_eqb2 n n1 n0 n2 t t0).
+    }
+    rewrite H in H1.
+    assert (eqb n n1 && eqb n0 n2 = true /\ args_eqb t t0 = true). apply andb_prop. assumption.
+    destruct H2.
+    assert (eqb n n1 = true /\ eqb n0 n2 = true). apply andb_prop; assumption.
+    destruct H4.
+    apply String.eqb_eq in H5. rewrite H5.
+    apply Nat.eqb_eq in H4. rename t into args1. rename t0 into args2.
+    rename n2 into nm.
+    induction args1.
+    + destruct args2. reflexivity. contradict H3. unfold args_eqb. discriminate.
+    + destruct args2. contradict H3; unfold args_eqb; discriminate.
+      Check args_eqb_ind.
+      
+      apply (args_eqb_ind n h h0 args1 args2) in H3 as H6.
+    assert (eqb n n1 = true). {
+      destruct H. unfold andb.
+    }
+  + assert ({v = v0} + {v <> v0}). { apply V_eq_dec. } destruct H0.
+    rewrite e; reflexivity.
+    contradiction.
+   destruct v; destruct v0. unfold eqb in H; unfold VEq in H. inversion H.
+    assert (Bool.reflect (n = n0) (n =? n0)). { apply eqb_spec. }
+    simpl; auto.
+    Compute (eqb_spec n n0).
+    apply eqb_spec in H1.
+     decide equality.
+   simpl; auto. unfold eqb in H; unfold EqTerm in H; unfold term_eqb in H. bdestruct (eqb v v0).
+  ++ 
+Qed.
+
+Lemma fun_eqb (n : nat) (s1 s2 : name) (args1 : Vector.t Term n) (args2 : Vector.t Term n) :
+  eqb (@Fun n s1 args1) (@Fun n s2 args2) = true <-> (s1 = s2 /\ args1 = args2).
+Proof.
+  intros.
+  split.
+  - intros. inversion H.
+    assert ((s1 =? s2) = true). {
+      unfold andb in H1; simpl; auto.
+      assert ((n =? n)%nat = true). apply Nat.eqb_refl.
+      rewrite H0 in H1.
+      destruct (s1 =? s2). reflexivity. discriminate.
+    }
+    assert ((n =? n)%nat = true). apply Nat.eqb_refl.
+    rewrite H0 in H1. rewrite H2 in H1. simpl in H1.
+    apply String.eqb_eq in H0.
+    split. assumption.
+    Check Vector.eqb_eq.
+    apply (Vector.eqb_eq Term term_eqb in H1. simpl; auto.
+
+Theorem term_dec (x y : Term) : {x = y} + {x <> y}.
+Proof.
+  intros. destruct (eqb x y) eqn:H.
+  - left. now apply eqb_eq.
+  decide equality. apply string_dec. 
+  decide equality.
+Qed.
+*)
+
+Lemma eq_dec : forall (x y : Term), {x = y} + {x <> y}. Admitted.
+
+(** *** Substitution Type Class
+
+We will want to substitute a term for a variable frequently in many syntactic
+constructs. Towards that end, we have a [Subst] type class.
+
+We may also want to do this with a vector of variables and a vector of terms,
+both vectors of the same length. Fortunately, we only have to define this
+"many-folded substitution" function only once.
+*)
+Class Subst A : Type := 
+{
+  subst : V -> Term -> A -> A
+}.
+
+Fixpoint subst_many {n} {A : Type} `{Subst A} (vars : Vector.t V n) (terms : Vector.t Term n) (a : A) : A :=
+match vars, terms with
+| x::xs, t::tms => subst_many xs (Vector.tl terms) (subst x t a)
+| _, _ => a
+end.
+
+(* HACK: since Coq cannot handle recursive typeclasses, we isolate the only
+recursive substitution here.
+
+See: https://stackoverflow.com/a/52349387 *)
+Fixpoint tsubst (x : V) (t : Term) (e : Term) : Term :=
+match e with
+| Var y => if eqb x y then t else e
+| @Fun n f args => @Fun n f (Vector.map (fun (a : Term) => tsubst x t a) args)
+| EConst _ => e
+end.
+
+Global Instance substTerm : Subst Term :=
+{
+  subst (x : V) (t : Term) (e : Term) := tsubst x t e
+}.
+
+Compute (subst (BVar 1) (Fun "c" []) (Fun "f" [Var (BVar 1) ; Var (FVar "x")])).
+
+Example term_subst_1 : subst (BVar 1) (Fun "c" []) (Fun "f" [Var (BVar 1) ; Var (FVar "x")])
+= Fun "f" [(Fun "c" []) ; Var (FVar "x")].
+Proof.
+  trivial.
+Qed.
+
+Example term_subst_2 : subst (FVar "x") (Fun "c" []) (Fun "f" [Var (BVar 1) ; Var (FVar "x")])
+= Fun "f" [Var (BVar 1) ; (Fun "c" [])].
+Proof.
+  trivial.
+Qed.
+
+Example term_subst_3 : subst (BVar 3) (Fun "c" []) (Fun "f" [Var (BVar 1) ; Var (FVar "x")])
+= Fun "f" [Var (BVar 1) ; Var (FVar "x")].
+Proof.
+  trivial.
+Qed.
+
+Example term_subst_4 : subst (FVar "z") (Fun "c" []) (Fun "f" [Var (BVar 1) ; Var (FVar "x")])
+= Fun "f" [Var (BVar 1) ; Var (FVar "x")].
+Proof.
+  trivial.
+Qed.
+
+Fixpoint term_map_var (f : V -> V) (t : Term) : Term :=
+match t with
+| Var x => Var (f x)
+| EConst _ => t
+| Fun nm args => Fun nm (Vector.map (fun (a : Term) => term_map_var f a) args)
+end.
+
+Lemma term_map_var_id : forall (t : Term),
+  term_map_var id t = t.
+Proof. intros. induction t.
+ (* apply Term_ind_mut.  dependent inversion t.  (fun (args : TermArgs) => (List.map (term_m.  *)
+  - simpl; auto.
+  - simpl; auto.
+  - rename t into args. 
+    assert(forall (t : Term), Vector.In t args -> ((fun t : Term => term_map_var id t = t) t)). {
+      apply Vector.Forall_forall. assumption.
+    }
+    assert (term_map_var id (Fun n0 args) = Fun n0 (Vector.map (fun (a : Term) => term_map_var id a) args)). {
+      unfold term_map_var; simpl; auto.
+    } rewrite H1.
+    simpl in H0.
+    assert (Vector.map (fun a : Term => term_map_var id a) args = args) as IH. {
+      induction args.
+      simpl; auto.
+      assert (Vector.map (fun a : Term => term_map_var id a) (h :: args)
+               = (term_map_var id h)::(Vector.map (fun a : Term => term_map_var id a) args)). {
+        unfold Vector.map; simpl; auto.
+      }
+      rewrite H2.
+      assert (term_map_var id h = h). {
+        apply H0. apply In_cons_hd.
+      }
+      rewrite H3.
+      assert (Vector.map (fun a : Term => term_map_var id a) args = args). { 
+        apply IHargs. simpl; auto. inversion H.
+        - apply Vector.Forall_forall.
+          assert (forall a : Term, VectorDef.In a args -> VectorDef.In a (h :: args)). {
+            intros. apply In_cons_tl. assumption.
+          }
+          intros.
+          simpl; auto.
+        - intros. assert (Vector.In t (h :: args)). apply In_cons_tl. assumption.
+          apply H0 in H5. assumption.
+        - simpl; auto.
+      }
+      rewrite H4. reflexivity.
+    }
+    rewrite IH. reflexivity.
+Qed.
+
+
+Fixpoint term_contains_bvar (index : nat) (t : Term) : Prop :=
+match t with
+| Var x => x = BVar index
+| EConst _ => False
+| @Fun n nm args => 
+  let fix args_contain_bvar {k} (ar : Vector.t Term k) :=
+     (match ar with
+      | Vector.nil _ => False
+      | Vector.cons _ h _ tl => term_contains_bvar index h \/ args_contain_bvar tl
+      end)
+  in args_contain_bvar args
+end.
+
+Class ContainsBVar A := {
+  contains_bvar : nat -> A -> Prop
+}.
+
+Global Instance ContainsBVarTerm : ContainsBVar Term := {
+  contains_bvar := term_contains_bvar
+}.
+
+Lemma term_subst_bvar_free : forall (n : nat) (t h : Term),
+  ~(contains_bvar n h) -> (subst (BVar n) t h) = h.
+Proof.
+  unfold contains_bvar; unfold ContainsBVarTerm. intros. induction h as [x|k|k nm args].
+  - destruct x.
+  + simpl; auto.
+  + unfold term_contains_bvar in H. simpl; auto.
+    assert (n0 <> n). { simpl; auto. }
+    bdestruct (Nat.eqb n n0).
+ ++ contradict H1; simpl; auto.
+ ++ reflexivity.
+  - simpl; auto.
+  - set (P := (fun h : Term => ~ term_contains_bvar n h -> subst (BVar n) t h = h)).
+    fold P in H0.
+    assert (forall (a : Term), VectorDef.In a args -> P a). {
+      apply Vector.Forall_forall. assumption.
+    }
+    assert(subst (BVar n) t (Fun nm args) = Fun nm (Vector.map (fun a : Term => tsubst (BVar n) t a) args)). {
+      simpl; auto.
+    } rewrite H2.
+    assert ((Vector.map (fun a : Term => tsubst (BVar n) t a) args) = args). {
+      induction args.
+      - simpl; auto.
+      - assert(Vector.map (fun a : Term => tsubst (BVar n) t a) (h :: args)%vector
+           = ((tsubst (BVar n) t h)::(Vector.map (fun a : Term => tsubst (BVar n) t a) args))%vector). {
+          simpl; auto.
+        }
+        rewrite H3.
+        assert(~ term_contains_bvar n (Fun nm (h :: args)%vector)
+                    -> ~ term_contains_bvar n (Fun nm args)). {
+          unfold term_contains_bvar; simpl; auto.
+        }
+        assert (Vector.Forall P args) as IH1. {
+          apply Vector.Forall_forall. intros; apply H1;
+            apply Vector.In_cons_tl; apply H5.
+        }
+        assert (~ term_contains_bvar n (Fun nm args)) as IH2. {
+          apply H4. apply H.
+        }
+        assert (forall a : Term, VectorDef.In a args -> P a) as IH3. {
+          intros. apply H1.  apply Vector.In_cons_tl; apply H5.
+        }
+        assert (subst (BVar n) t (Fun nm args) =
+                Fun nm (Vector.map (fun a : Term => tsubst (BVar n) t a) args)). {
+          unfold subst; simpl; auto.
+        }
+        assert((Vector.map (fun a : Term => tsubst (BVar n) t a) args) = args). {
+          apply IHargs. simpl; auto. simpl; auto. simpl; auto. simpl; auto.
+        } rewrite H6.
+        clear IH1 IH2 IH3 H6.
+        assert (tsubst (BVar n) t h = h). {
+          assert (P h). {
+            apply H1. apply Vector.In_cons_hd.
+          }
+          unfold P in H6. unfold subst in H6; unfold substTerm in H6.
+          apply H6.
+          assert (~ term_contains_bvar n (Fun nm (h :: args)%vector) -> ~ term_contains_bvar n h). {
+            simpl; auto.
+          }
+          apply H7. apply H.
+        }
+        rewrite H6. reflexivity.
+    }
+    rewrite H3. reflexivity.
+Qed.
+
+(*
+Definition tlift (c d : nat) (t : Term) := term_map_var (lift c d) t.
+
+Fixpoint tlift (c d : nat) (t : Term) : Term :=
+match t with
+| Var y => Var (lift c d y)
+| Fun f args => Fun f (Vector.map (fun (a : Term) => tlift c d a) args)
+| EConst _ => t
+end.
+*)
+
+Global Instance liftTerm : Lift Term :=
+{
+  lift (c d : nat) (t : Term) := term_map_var (lift c d) t
+}.
+
+Definition tlift := lift.
+(* (c d : nat) (t : Term) := term_map_var (lift c d) t. *)
+
+(** Lemma: [lift 0 0] is the identity transformation. *)
+Lemma term_zero_lift_is_id : forall (t : Term), lift 0 0 t = id t.
+Proof.
+  intros. induction t.
+  - assert (@lift V VLift 0 0 = id). apply zero_lift_is_id.
+    unfold lift; unfold liftTerm. rewrite H. 
+    assert (id (Var v) = Var v). { unfold id; simpl; auto. }
+    assert (@lift V VLift 0 0 v = id v). {
+      apply equal_f. trivial.
+    }
+    unfold term_map_var. unfold id. reflexivity.
+  - unfold lift; unfold term_map_var; simpl; auto.
+  - rename t into args.
+    set (P := (fun t : Term => lift 0 0 t = id t)). fold P in H.
+    assert (forall a : Term, VectorDef.In a args -> P a). {
+      apply (Vector.Forall_forall Term P n args). assumption.
+    }
+    
+    assert (lift 0 0 (Fun n0 args) = Fun n0 (Vector.map (fun a : Term => term_map_var (lift 0 0) a) args)). {
+      unfold lift; unfold liftTerm; unfold term_map_var; simpl; auto.
+    } rewrite H1. clear H1.
+    assert (Vector.map (fun a : Term => term_map_var (lift 0 0) a) args = args). {
+      admit.
+    }
+    rewrite H1. unfold id. reflexivity.
+Admitted.
+
+Definition term_is_fun (t : Term) : Prop :=
+  match t with
+  | Fun _ _ =>  True
+  | _ => False
+  end.
+
+Class Fresh A : Type := {
+  fresh : Term -> A -> Prop
+}.
+
+Fixpoint fresh_term (c : Term) (t : Term) : Prop :=
+match t, c with
+| Var x, Var y => x <> y
+| EConst m, EConst n => m <> n
+| Fun f args1, Fun g args2 => t <> c /\
+  let fix fresh_args {k} (ars : Vector.t Term k) :=
+          match ars with
+          | tm::ars1 => (fresh_term c tm) /\ fresh_args ars1
+          | [] => True
+          end
+  in fresh_args args1
+| _,_ => True
+end.
+
+Global Instance FreshTerm : Fresh Term := {
+  fresh := fresh_term
+}.
+
+(** ** New Existential Variables 
+
+We can assemble the list of existential variables appearing in a
+[Term], [Formula], whatever. Then we can generate a fresh
+existential variable.
+*)
+
+Class EnumerateEVars A := {
+  list_evars : A -> list nat
+}.
+
+Fixpoint list_evars_term (t : Term) (l : list nat) : list nat :=
+match t with
+| Var _ => l
+| EConst n => insert n l
+| Fun f args => Vector.fold_left (fun l' => fun (arg : Term) => insert_merge (list_evars_term arg l') l')
+    l args
+end.
+
+Theorem list_evars_term_sorted : forall (t : Term) (l : list nat),
+  sorted l -> sorted (list_evars_term t l).
+Proof.
+  intros.
+  induction t.
+  - assert (list_evars_term (Var v) l = l). { simpl; auto. }
+    rewrite H0. assumption.
+  - assert (list_evars_term (EConst n) l = insert n l). { simpl; auto. }
+    rewrite H0. apply insert_preserves_sorted. assumption.
+  - rename t into args.
+    assert (list_evars_term (Fun n0 args) l = Vector.fold_left (fun l' => fun (arg : Term) => insert_merge (list_evars_term arg l') l')
+    l args). { simpl; auto. }
+    rewrite H1. apply insert_merge_vector_fold_sorted2.
+    assumption.
+Qed.
+
+Global Instance EnumerateEVarsTerm : EnumerateEVars Term := {
+  list_evars tm := list_evars_term tm []
+}.
+
+Theorem list_evers_term_sorted : forall (t : Term),
+  sorted (list_evars t).
+Proof. intros.
+  unfold list_evars; unfold EnumerateEVarsTerm.
+  assert (sorted []%list). { apply sorted_nil. }
+  apply list_evars_term_sorted.
+  assumption.
+Qed.
+
+(** The alternate approach is that fresh existential variables will be [0],
+and when we introduce one, we [shift_evars] in the related formulas. *)
+Class ShiftEvars A := {
+  shift_evars : A -> A
+}.
+
+Fixpoint shift_evars_term (t : Term) : Term :=
+match t with
+| Var _ => t
+| EConst n => EConst (S n)
+| Fun f args => Fun f (Vector.map shift_evars_term args)
+end.
+
+Global Instance ShiftEvarsTerm : ShiftEvars Term := {
+shift_evars := shift_evars_term
+}.
