ST/Logic/V.v
@@ -1,0 +1,195 @@
+Require Import String.
+Require Import Lia.
+Require Import List.
+Require Import Nat.
+Require Import Coq.Vectors.Vector.
+Require Export Coq.Arith.Compare_dec.
+Require Import Coq.Arith.PeanoNat.
+Require Import Coq.Arith.Peano_dec.
+Require Import Coq.Logic.Classical_Prop.
+Require Import Coq.Logic.FunctionalExtensionality.
+From ST Require Import EVarsScratchwork.
+Import ListNotations.
+Import VectorNotations.
+Open Scope string_scope.
+
+(* TODO: re-do the local context so that it meshes with locally nameless
+variables correctly. *)
+
+(** * Introduction
+
+We have a couple of helper type classes for recurring functions expected on
+constructs, things like [eqb] for boolean equality testing, and [subst] for
+substituting a [Term] for a [V]ariable.
+*)
+
+(** Exercise #1.
+Extend this definition to make [eqb] a proper equivalence relation, specifically:
+
+- [eqb_refl : forall (a : A), eqb a a = true]
+- [eqb_sym : forall (a b : A), eqb a b = eqb b a]
+- [eqb_trans : forall (a b c : A), eqb a b = eqb b c -> eqb a c]
+
+Exercise #2.
+Extend this definition to include
+- [eqb_eq : forall (a b : A), eqb a b = true <-> a = b]
+- [eqb_neq : forall (a b : A), eqb a b = false <-> a <> b] 
+*)
+Class Eq A :=
+  {
+    eqb: A -> A -> bool;
+  }.
+
+Fixpoint list_eqb {A : Type} (v1 v2 : list A) (eq : A -> A -> bool) : bool :=
+  match v1,v2 with
+  | List.nil, List.nil => true
+  | List.cons h1 t1, List.cons h2 t2 => andb (eq h1 h2) (list_eqb t1 t2 eq)
+  | _, _ => false
+  end.
+
+Global Instance natEq : Eq nat := {
+  eqb (n1 n2 : nat) := Nat.eqb n1 n2
+}.
+
+Global Instance stringEq : Eq string := {
+  eqb := String.eqb
+}.
+
+(** * Soft Type System
+
+We begin formalizing our soft type system by defining variables and terms,
+and the other syntactic constructs. Then we will inductively define the rules
+of inference for the soft type system.
+
+** Names and Variables
+
+We use locally nameless encoding of bound variables. Free variables are any
+arbitrary [name] instances. Bound variables are de Bruijn indices.
+*)
+
+Definition name : Type := string.
+
+Inductive V :=
+| FVar : name -> V
+| BVar : nat -> V.
+
+Theorem var_dec (x y : V) : {x = y} + {x <> y}.
+Proof.
+  decide equality. apply string_dec. 
+  decide equality.
+Qed.
+
+Global Instance VEq : Eq V := {
+  eqb (x y : V) :=
+  match x, y with
+  | FVar s1, FVar s2 => eqb s1 s2
+  | BVar n1, BVar n2 => eqb n1 n2
+  | _, _ => false
+  end
+}.
+
+Lemma V_eqb_refl : forall a : V, eqb a a = true.
+Proof.
+  intros. destruct a.
+  - unfold eqb; unfold VEq. simpl; auto. apply String.eqb_refl.
+  - unfold eqb; unfold VEq. simpl; auto. apply Nat.eqb_refl.
+Qed.
+
+Lemma V_eq_dec : forall a b : V, {a = b} + {a <> b}.
+Proof. decide equality.
+  try (left; reflexivity); try (right; congruence).
+  - apply string_dec.
+  - decide equality.
+Defined.
+
+Theorem easy : forall p q:Prop, (p->q)->(~q->~p).
+Proof.
+  intros. intro. apply H0. apply H. exact H1. 
+Qed.
+
+Lemma PPNN : forall p:Prop, p -> ~ ~ p.
+Proof.
+  unfold not; intros; elim (classic p); auto.
+Qed.
+
+Theorem contra  : forall p q:Prop, (~q->~p) -> (p->q).
+Proof. intros. 
+  apply (easy (~q) (~p)) in H.
+  apply NNPP in H. assumption. apply PPNN; assumption. 
+Qed.
+
+Lemma V_eqb_eq : forall a b : V, eqb a b = true <-> a = b.
+Proof.
+  intros. split.
+  - intros. destruct a.
+  + unfold eqb in H; unfold VEq in H. destruct b. apply String.eqb_eq in H.
+    rewrite H; reflexivity. discriminate H.
+  + unfold eqb in H; unfold VEq in H. destruct b. discriminate.
+    apply Nat.eqb_eq in H.
+    rewrite H; reflexivity.
+  - intros. rewrite H; apply V_eqb_refl.
+Qed.
+
+(** We now need to handle [lift]-ing a bound variable. Since this will occur
+wherever a [BVar] can occur (and wherever a [Term] may occur), we will use a
+typeclass to handle this. *)
+
+Class Lift A := {
+  lift : nat -> nat -> A -> A
+}.
+
+Definition shift {A : Type} `{Lift A} (a : A) : A := lift 0 1 a.
+Global Instance VLift : Lift V := {
+  lift (cutoff depth : nat) (x : V) :=
+  match x with
+  | FVar nm => x
+  | BVar n => if (* lt_dec n cutoff *) Nat.ltb n cutoff then x else BVar (n+depth)
+  end
+}.
+
+(** Lemma: [lift 0 0] is the identity transformation.
+Lemma zero_lift_is_id0 : forall (n : nat), lift 0 0 (BVar n) = (BVar n).
+Proof.
+  intros. simpl. auto.
+Qed.
+Lemma zero_lift_is_id : forall (x : V), lift 0 0 x = x.
+Proof.
+  intros. destruct x.
+  - simpl; auto.
+  - simpl; auto.
+Qed.
+ *)
+
+
+Lemma zero_lift_is_id :  lift 0 0 = id.
+Proof.
+  apply functional_extensionality.
+  intros. destruct x.
+  - simpl; auto.
+  - simpl; auto. assert (n + 0 = n). { lia. } rewrite H. unfold id. reflexivity.
+Qed.
+
+
+Theorem case_lift_is_not_id : forall (i k n : nat), n >= k -> lift k i (BVar n) = BVar (n+i).
+Proof.
+  intros. simpl. bdestruct (Nat.ltb n k).
+  - contradict H. lia.
+  - reflexivity.
+Qed.
+
+Theorem case_lift_is_id : forall (i k n : nat), n < k -> lift k i (BVar n) = BVar (n).
+Proof.
+  intros. simpl. bdestruct (Nat.ltb n k).
+  - reflexivity.
+  - contradict H. lia.
+Qed.
+
+Example shift_is_not_id : shift (BVar 0) = (BVar 1).
+Proof.
+  trivial.
+Qed.
+
+Example shift_really_shifts : forall (n : nat), shift (BVar n) = BVar (n + 1).
+Proof.
+  trivial.
+Qed.
